<rdf:RDF xmlns:rdf="http://www.w3.org/1999/02/22-rdf-syntax-ns#" 
	xmlns:rdfs="http://www.w3.org/2000/01/rdf-schema#" 
	xmlns:dc="http://purl.org/dc/elements/1.1/" 
	xmlns:rss="http://purl.org/rss/1.0/"
	xmlns:owl="http://www.w3.org/2002/07/owl#"
	xmlns:attach="http://wymiwyg.org/ontologies/rss/attach#" 
	xml:base="http://wymiwyg.org/ontologies/rss/attach">
	<!--  Class declarations   -->
	<owl:Ontology rdf:about="" dc:title="RSS Attachment module"/>
	<rdfs:Class rdf:ID="Attachment" rdfs:label="Attachment" 
		rdfs:comment="Describes an attachment, attachment is a reference to another document
		with infomation on how this is to be included to the document to which it is attached.
		An attachment may have a rdfs:label, a dc:language and a rdfs:comment">
		<rdfs:isDefinedBy rdf:resource="http://wymiwyg.org/ontologies/rss/attach"/>
	</rdfs:Class>
	<rdfs:Class rdf:ID="InlineAttachment" rdfs:label="InlineAttachment" 
		rdfs:comment="Describes an attachment that should be displayed inline">
		<rdfs:subClassOf rdf:resource="#Attachment"/>
		<rdfs:isDefinedBy rdf:resource="http://wymiwyg.org/ontologies/rss/attach"/>
	</rdfs:Class>
	<rdfs:Class rdf:ID="SummaryAttachment" rdfs:label="SummaryAttachment" 
		rdfs:comment="Describes an attachment that should be (also) be displaied
		 when showing the article in summary-mode">
		<rdfs:subClassOf rdf:resource="#Attachment"/>
		<rdfs:isDefinedBy rdf:resource="http://wymiwyg.org/ontologies/rss/attach"/>
	</rdfs:Class>
	<!--  Property declarations   -->
	<rdf:Property rdf:ID="attachments" rdfs:label="Attachments" 
		rdfs:comment="A sequence of attachments attached to an item">
		<rdfs:range rdf:resource="http://www.w3.org/1999/02/22-rdf-syntax-ns#Seq"/>
		<rdfs:isDefinedBy rdf:resource="http://wymiwyg.org/ontologies/rss/attach"/>
	</rdf:Property>
	<rdf:Property rdf:ID="document" rdfs:label="document" 
		rdfs:comment="The attached document, the URI of the object of this property must be dereferenceable">
		<rdfs:domain rdf:resource="#Attachment"/>
		<rdfs:isDefinedBy rdf:resource="http://wymiwyg.org/ontologies/rss/attach"/>
	</rdf:Property>
	<rdf:Property rdf:ID="height" rdfs:label="height" 
		rdfs:comment="The height of an image.">
		<rdfs:domain rdf:resource="#InlineAttachment"/>
		<rdfs:isDefinedBy rdf:resource="http://wymiwyg.org/ontologies/rss/attach"/>
	</rdf:Property>
	<rdf:Property rdf:ID="width" rdfs:label="width" 
		rdfs:comment="The width of an image.">
		<rdfs:domain rdf:resource="#InlineAttachment"/>
		<rdfs:isDefinedBy rdf:resource="http://wymiwyg.org/ontologies/rss/attach"/>
	</rdf:Property>
	<rdf:Property rdf:ID="type" rdfs:label="type" 
		rdfs:comment="The (preffered) media-type the refernced document should be included 
		(i.e. the first accept-header value the client should set when requesting the resource with http)">
		<rdfs:domain rdf:resource="#InlineAttachment"/>
		<rdfs:isDefinedBy rdf:resource="http://wymiwyg.org/ontologies/rss/attach"/>
	</rdf:Property>
</rdf:RDF>