<!-- this is an incomplete draft, it contains modification to Kevin's original proposal -->

<rdf:RDF 
     xmlns:rdf="http://www.w3.org/1999/02/22-rdf-syntax-ns#" 
     xmlns:rdfs="http://www.w3.org/2000/01/rdf-schema#"
     xmlns:dc="http://purl.org/dc/elements/1.1/"
     xmlns:rss="http://purl.org/rss/1.0/"
     xmlns:l="http://wymiwyg.org/ontologies/rss/link#"
     xml:base="http://wymiwyg.org/ontologies/rss/link">

 <!--  Class declarations   --> 

 <rdfs:Class rdf:ID="Link"
   rdfs:label="Link"
   rdfs:comment="Describes a link.">
   <rdfs:isDefinedBy rdf:resource="http://wymiwyg.org/ontologies/rss/link#" /> 
 </rdfs:Class>
 
 <rdfs:Class rdf:ID="Topic"
   rdfs:label="Topic">
   <rdfs:comment>This type of link provides a link to the current RSS channel or item by topic. 
   This is generally an HTML or RSS file which contains RSS items on the same 
   topic as the current item/channel.</rdfs:comment>
   <rdfs:subClassOf
   rdf:resource="#Link"/>
   <rdfs:isDefinedBy rdf:resource="http://wymiwyg.org/ontologies/rss/link#" /> 
 </rdfs:Class>
 
 <rdfs:Class rdf:ID="SubChannel"
   rdfs:label="SubChannel">
   <rdfs:comment>This type of link provides a link to a subchannel of the current channel. The
   target of the Link is subordinated to this channel.</rdfs:comment>
   <rdfs:subClassOf
   rdf:resource="#Link"/>
   <rdfs:isDefinedBy rdf:resource="http://wymiwyg.org/ontologies/rss/link#" /> 
 </rdfs:Class>
 
 <rdfs:Class rdf:ID="Container"
   rdfs:label="Container">
   <rdfs:comment>This links an item or channel to a channel which "contains" the item.</rdfs:comment>
   <rdfs:subClassOf
   rdf:resource="#Link"/>
   <rdfs:isDefinedBy rdf:resource="http://wymiwyg.org/ontologies/rss/link#" /> 
 </rdfs:Class>
 
 <rdfs:Class rdf:ID="Language"
   rdfs:label="Language">
   <rdfs:comment>This type of link provides a link to other language version of this channel. Resource of this type usually have the dc:language and the link:target attribute.</rdfs:comment>
   <rdfs:subClassOf
   rdf:resource="#Link"/>
   <rdfs:isDefinedBy rdf:resource="http://wymiwyg.org/ontologies/rss/link#" /> 
 </rdfs:Class>
 
  <!--  Property declarations   --> 

 <rdf:Property rdf:ID="link"
   rdfs:label="link"
   rdfs:comment="A property of item or channel with an instance of Link as value.">
   <rdfs:range rdf:resource="Link"/> 
   <rdfs:isDefinedBy rdf:resource="http://wymiwyg.org/ontologies/rss/link#" /> 
 </rdf:Property>
 
 <rdf:Property rdf:ID="linkedBy"
   rdfs:label="linkedBy"
   rdfs:comment="The inverse property of link.">
   <rdfs:domain rdf:resource="Link"/> 
   <rdfs:isDefinedBy rdf:resource="http://wymiwyg.org/ontologies/rss/link#" /> 
 </rdf:Property>
 
 <rdf:Property rdf:ID="links"
   rdfs:label="links"
   rdfs:comment="A property of item or channel with an Sequence of Links as value.">
   <rdfs:range rdf:resource="http://www.w3.org/1999/02/22-rdf-syntax-ns#Seq"/> 
   <rdfs:isDefinedBy rdf:resource="http://wymiwyg.org/ontologies/rss/link#" /> 
 </rdf:Property>

 <rdf:Property rdf:ID="target"
    rdfs:label="target"
    rdfs:comment="The target of a link.">
   <rdfs:domain rdf:resource="Link"/> 
   <rdfs:range rdf:resource="http://www.w3.org/2000/01/rdf-schema#Resource"/> 
   <rdfs:isDefinedBy rdf:resource="http://wymiwyg.org/ontologies/rss/link/" /> 
 </rdf:Property>
 
 <rdf:Property rdf:ID="targetOf"
    rdfs:label="targetOf"
    rdfs:comment="The inverse property of target.">
   <rdfs:domain rdf:resource="http://www.w3.org/2000/01/rdf-schema#Resource"/>
	 <rdfs:range rdf:resource="Link"/>
   <rdfs:isDefinedBy rdf:resource="http://wymiwyg.org/ontologies/rss/link/" /> 
 </rdf:Property>

</rdf:RDF>