
<rdf:RDF xmlns:rdf="http://www.w3.org/1999/02/22-rdf-syntax-ns#"
		xmlns:rdfs="http://www.w3.org/2000/01/rdf-schema#"
		xmlns:owl="http://www.w3.org/2002/07/owl#"
		xmlns="http://wymiwyg.org/ontologies/foaf/role#"
		xml:base="http://wymiwyg.org/ontologies/foaf/role">

	<owl:Ontology rdf:about="">
		<rdfs:comment xml:lang="en">An ontology for describing roles and participations. A participation
		is an Agent in a Group, a Role is an individual-independent function a group provides.</rdfs:comment>
	</owl:Ontology>
	
	<rdfs:Class rdf:ID="Role">
		<rdfs:label xml:lang="en">Role</rdfs:label>
		<rdfs:comment xml:lang="en">Describes a Role (Function/Position) agents may have within a Group, a Role is
		associated to exactly one group, so the role of the Chief-Idologist of on group is never
		the same resource as the Chief-Ideologist of another group. Multiple Particpations may howere have the same role.
		The rdfs:label should be used
		to indicate the denotation of the role (like "Chief Ideologist"), the foaf:name property
		may be used to indicate how a holder of this role may be referred to, e.g. "Chief Ideologist of WYMIWYG.org".</rdfs:comment>
		<rdfs:subClassOf rdf:resource="http://xmlns.com/foaf/0.1/Agent"/>
	</rdfs:Class>

	<rdfs:Class rdf:ID="Participation">
		<rdfs:label xml:lang="en">Participation</rdfs:label>
		<rdfs:comment xml:lang="en">Describes that and in which Role an Agent participates in a group. The
		group is indicated by the group property (exactly 1), the participant by the participant property
		(excatly 1), and an arbitrary number of roles with the exposesRole property. Note that a participation may
		only have roles that belong to the respective group, i.e. which have the same group property.</rdfs:comment>
		<rdfs:subClassOf rdf:resource="http://xmlns.com/foaf/0.1/Agent"/>
	</rdfs:Class>

	<rdf:Property rdf:ID="participatesIn">
		<rdfs:label xml:lang="en">participates in</rdfs:label>
		<rdfs:label xml:lang="de">partizipiert in</rdfs:label>
		<rdfs:comment xml:lang="en">Indicates a participation of the subject</rdfs:comment>
		<owl:inverseOf rdf:resource="#participant"/>
		<rdfs:domain rdf:resource="http://xmlns.com/foaf/0.1/Agent"/>
		<rdfs:range rdf:resource="#Participation"/>
	</rdf:Property>

	<rdf:Property rdf:ID="participant">
		<rdfs:label xml:lang="en">participant</rdfs:label>
		<rdfs:label xml:lang="de">TeilnehmerIn</rdfs:label>
		<rdfs:comment xml:lang="en">Indicates the particpant in the participation described by the subject</rdfs:comment>
		<owl:inverseOf rdf:resource="#participates"/>
		<rdfs:range rdf:resource="http://xmlns.com/foaf/0.1/Agent"/>
		<rdfs:domain rdf:resource="#Participation"/>
	</rdf:Property>
	
	<rdf:Property rdf:ID="group">
		<rdfs:label xml:lang="en">Group</rdfs:label>
		<rdfs:label xml:lang="de">Gruppe</rdfs:label>
		<rdfs:comment xml:lang="en">Indicates the group in which the participation described 
		by the subject takes place</rdfs:comment>
		<rdfs:domain>
			<owl:Class>
				<owl:unionOf rdf:parseType="Collection">
					<owl:Class rdf:about="#Participation" />
					<owl:Class rdf:about="#Role" />
				</owl:unionOf>
			</owl:Class>
		</rdfs:domain>
		<rdfs:range rdf:resource="http://xmlns.com/foaf/0.1/Group"/>
		<owl:inverseOf rdf:resource="#hasParticipation"/>
	</rdf:Property>
	
	<rdf:Property rdf:ID="hasParticipation">
		<rdfs:label xml:lang="en">has participation</rdfs:label>
		<rdfs:label xml:lang="de">hat Teilnahme</rdfs:label>
		<rdfs:range rdf:resource="#Participation"/>
		<rdfs:domain rdf:resource="http://xmlns.com/foaf/0.1/Group"/>
		<owl:inverseOf rdf:parseType="Resource"> 
			<rdfs:subclassOf rdf:resource="#group"/>
		</owl:inverseOf>
	</rdf:Property>

	<rdf:Property rdf:ID="actsInRole">
		<rdfs:label xml:lang="en">acts as role</rdfs:label>
		<rdfs:label xml:lang="de">agiert in der Rolle</rdfs:label>
		<rdfs:comment xml:lang="en">The role of the participipation in the group. This role must have
		the same group as the subject.</rdfs:comment>
		<rdfs:domain rdf:resource="#Participation"/>
		<rdfs:range rdf:resource="#Role"/>
	</rdf:Property>
	
	<rdf:Property rdf:ID="providesRole">
		<rdfs:label xml:lang="en">provides role</rdfs:label>
		<rdfs:label xml:lang="de">sieht Rolle vor</rdfs:label>
		<rdfs:comment xml:lang="en">A role a group provieds, i.e. a role that participations in a group may act in.</rdfs:comment>
		<rdfs:domain rdf:resource="#Participation"/>
		<rdfs:range rdf:resource="#Role"/>
	</rdf:Property>

</rdf:RDF>